HepLean/PerturbationTheory/Contractions/Involutions.lean
@@ -30,11 +30,11 @@ def toInvolution : {f : Fin n → Fin n // Function.Involutive f} :=
 def fromInvolution (f : {f : Fin n → Fin n // Function.Involutive f}) : ContractionsNat n :=
   ⟨Finset.univ.filter (fun a => a.card = 2 ∧ ∃ i, {i, f.1 i} = a), by
   intro a
-  simp
+  simp only [Finset.mem_filter, Finset.mem_univ, true_and, and_imp, forall_exists_index]
   intro h1 _ _
   exact h1, by
   intro a ha b hb
-  simp at ha hb
+  simp only [Finset.mem_filter, Finset.mem_univ, true_and] at ha hb
   obtain ⟨i, hai⟩ := ha.2
   subst hai
   obtain ⟨j, hbj⟩ := hb.2
@@ -44,11 +44,13 @@ def fromInvolution (f : {f : Fin n → Fin n // Function.Involutive f}) : Contra
     simp
   · by_cases hi : i = f.1 j
     · subst hi
-      simp
+      simp only [Finset.disjoint_insert_right, Finset.mem_insert, Finset.mem_singleton, not_or,
+        Finset.disjoint_singleton_right, true_or, not_true_eq_false, and_false, or_false]
       rw [f.2]
       rw [@Finset.pair_comm]
     · apply Or.inr
-      simp
+      simp only [Finset.disjoint_insert_right, Finset.mem_insert, Finset.mem_singleton, not_or,
+        Finset.disjoint_singleton_right]
       apply And.intro
       · apply And.intro
         · exact fun a => h a.symm
@@ -70,7 +72,7 @@ lemma fromInvolution_getDual?_isSome (f : {f : Fin n → Fin n // Function.Invol
   · intro h
     obtain ⟨a, ha⟩ := h
     have ha2 := a.2
-    simp [fromInvolution, -Finset.coe_mem] at ha2
+    simp only [fromInvolution, Finset.mem_filter, Finset.mem_univ, true_and] at ha2
     obtain ⟨j, h⟩ := ha2.2
     rw [← h] at ha
     have hj : f.1 j ≠ j := by
@@ -78,7 +80,7 @@ lemma fromInvolution_getDual?_isSome (f : {f : Fin n → Fin n // Function.Invol
       rw [hn] at h
       rw [← h] at ha2
       simp at ha2
-    simp at ha
+    simp only [Finset.mem_insert, Finset.mem_singleton] at ha
     rcases ha with ha | ha
     · subst ha
       exact hj
@@ -87,7 +89,8 @@ lemma fromInvolution_getDual?_isSome (f : {f : Fin n → Fin n // Function.Invol
       exact id (Ne.symm hj)
   · intro hi
     use ⟨{i, f.1 i}, by
-      simp [fromInvolution]
+      simp only [fromInvolution, Finset.mem_filter, Finset.mem_univ, exists_apply_eq_apply,
+        and_true, true_and]
       rw [Finset.card_pair (id (Ne.symm hi))]⟩
     simp
 
@@ -95,9 +98,10 @@ lemma fromInvolution_getDual?_eq_some (f : {f : Fin n → Fin n // Function.Invo
     (h : ((fromInvolution f).getDual? i).isSome) :
     ((fromInvolution f).getDual? i) = some (f.1 i) := by
   rw [@getDual?_eq_some_iff_mem]
-  simp [fromInvolution]
+  simp only [fromInvolution, Finset.mem_filter, Finset.mem_univ, exists_apply_eq_apply, and_true,
+    true_and]
   apply Finset.card_pair
-  simp at h
+  simp only [fromInvolution_getDual?_isSome, ne_eq] at h
   exact fun a => h (id (Eq.symm a))
 
 @[simp]
@@ -109,22 +113,22 @@ lemma fromInvolution_getDual?_get (f : {f : Fin n → Fin n // Function.Involuti
 
 lemma toInvolution_fromInvolution : fromInvolution c.toInvolution = c := by
   apply Subtype.eq
-  simp [fromInvolution, toInvolution]
+  simp only [fromInvolution, toInvolution]
   ext a
-  simp
+  simp only [Finset.mem_filter, Finset.mem_univ, true_and]
   apply Iff.intro
   · intro h
     obtain ⟨i, hi⟩ := h.2
     split at hi
     · subst hi
       simp
-    · simp at hi
+    · simp only [Finset.mem_singleton, Finset.insert_eq_of_mem] at hi
       subst hi
       simp at h
   · intro ha
     apply And.intro (c.2.1 a ha)
     use c.fstFieldOfContract ⟨a, ha⟩
-    simp
+    simp only [fstFieldOfContract_getDual?, Option.isSome_some, ↓reduceDIte, Option.get_some]
     change _ = (⟨a, ha⟩ : c.1).1
     conv_rhs => rw [finset_eq_fstFieldOfContract_sndFieldOfContract]
 
@@ -137,7 +141,7 @@ lemma fromInvolution_toInvolution (f : {f : Fin n → Fin n // Function.Involuti
   · rename_i h
     simp
   · rename_i h
-    simp at h
+    simp only [fromInvolution_getDual?_isSome, ne_eq, Decidable.not_not] at h
     exact id (Eq.symm h)
 
 def equivInvolution : ContractionsNat n ≃ {f : Fin n → Fin n // Function.Involutive f} where
